Tests for state handlers

Tests.v
@@ -4,18 +4,27 @@ From Coq Require Import Strings.String.
 From Freak Require Import Language.
 From Freak Require Import Map.
 From Freak Require Import Semantics.
+From Freak Require Import Opt.
 
 Module Tests.
 
 Definition rnat x := <{ return x }>.
+Definition rtrue := <{ return true }>.
 Definition x : string := "x".
 Definition y : string := "y".
 Definition s : string := "s".
+Definition s' : string := "s'".
 Definition f : string := "f".
 Definition p : string := "p".
 Definition k : string := "k".
+Definition k' : string := "k'".
 Definition Const : string := "Const".
+Definition Put : string := "Put".
+Definition coalgPutGet : string := "_coalg_Put_Get".
+Definition Get : string := "Get".
 Hint Unfold rnat : core.
+
+(* Test lambda calculus *)
 
 Example eval_nat: rnat 42 -->* rnat 42.
 Proof. normalize. Qed.
@@ -58,6 +67,7 @@ Example static_scope :
   }> -->* rnat 1.
 Proof. normalize. Qed.
 
+(* Test handlers *)
 
 Example trivial_handler :
   <{ handle return 1 with ( |r #return x -> return x ) }>
@@ -80,6 +90,68 @@ Proof.
     eapply multi_step.
     - eapply step_handle_op. simpl. auto. auto.
     - normalize.
+Qed.
+
+Definition state_handler : handler := <{
+    |o # Put , s' , k |-> return (\s ->
+         let k' <- k true in k' s'
+    );
+
+    |o # Get , s' , k |-> return (\s ->
+         let k' <- k s in k' s
+    );
+    |r #return x -> return (\s -> return x)
+  }>.
+
+Example state_handler_get_initial :
+  <{ let f <- handle
+        do x <- Get @ true in
+        return x
+    with state_handler
+    in f 1
+  }>
+  -->* rnat 1.
+Proof.
+    unfold state_handler.
+    eapply multi_step.
+    - apply step_let. eapply step_handle_op. simpl. auto. auto.
+    - normalize.
+Qed.
+
+Example state_handler_put :
+  <{ let f <- handle
+        do y <- Put @ 2 in return y
+    with state_handler
+    in f 1
+  }>
+  -->* rtrue.
+Proof.
+    unfold state_handler.
+    eapply multi_step.
+    - apply step_let. eapply step_handle_op. simpl. auto. auto.
+    - simpl. normalize.
+Qed.
+
+Example state_handler_put_get :
+  <{ let f <- handle
+        do y <- Put @ 2 in
+        do x <- Get @ true in
+        return x
+    with state_handler
+    in f 1
+  }>
+  -->* rnat 2.
+Proof.
+    unfold state_handler.
+    eapply multi_step.
+    - apply step_let.  eapply step_handle_op. simpl. auto. auto.
+    - simpl.
+      eapply multi_step. auto. simpl.
+      eapply multi_step. auto. simpl.
+      eapply multi_step. auto. simpl.
+      eapply multi_step.
+      apply step_let. apply step_handle_op. simpl. auto. auto.
+      simpl. normalize.
 Qed.
 
 End Tests.
